@prefix dcat:   <http://www.w3.org/ns/dcat#> .
@prefix dct:     <http://purl.org/dc/terms/> .
@prefix xsd:    <http://www.w3.org/2001/XMLSchema#> .
@prefix foaf:   <http://xmlns.com/foaf/0.1/> .
@prefix vcard:  <http://www.w3.org/2006/vcard/ns#> .
@prefix adms:   <http://www.w3.org/ns/adms> .
@prefix schema: <http://schema.org/> .
@prefix dcatap: <http://data.europa.eu/r5r/> .
@prefix skos:   <http://www.w3.org/2004/02/skos/core#> .

<https://doi.org/10.5281/zenodo.6984525>  
    a dcat:Dataset ;
    dct:description "This dataset contains crowdsourced image descriptions for 7543 images from the DEArt dataset. There are 4-5 descriptions per image, provided by volunteers of the Zooniverse crowdsourcing platform. The guidelines we used, together with some examples of possible captions, are also published in Zooniverse.  We are in debt with all the Zooniverse volunteers and coordinators, and in particular with Samantha Blickhan, for making this possible. The dataset is a data export from Zooniverse in CSV format, in which the user information has been anonymized."@en ; 
    dct:title "Image descriptions for 7543 of the DEArt images, obtained via the Zooniverse crowdsourcing platform"@en ;
    dct:publisher <https://saintgeorgeonabike.eu/> ;
	dcat:contactPoint <https://saintgeorgeonabike.eu/> ;
	dct:accessRights <http://publications.europa.eu/resource/authority/access-right/PUBLIC> ;
    dcat:theme <http://publications.europa.eu/resource/authority/data-theme/EDUC> ;
    dct:creator <https://saintgeorgeonabike.eu/> ;
    dct:temporal [
		a dct:PeriodOfTime;
		dcat:startDate "1101-01-01"^^xsd:date ;
		dcat:endDate "1800-12-31"^^xsd:date 
    ] ;
    dct:spatial <http://publications.europa.eu/resource/authority/continent/EUROPE> ;
#   dct:issued "2023-01-01"^^xsd:date ;
#	dct:modified "2023-01-01"^^xsd:date ;
    dcat:keyword "Visual Content Description"@en , "2D Art"@en , "Cultural Heritage"@en , "Crowdsourcing"@en  ;	
    foaf:page <https://help.zooniverse.org/next-steps/data-exports/> , <https://www.zooniverse.org/projects/artem-dot-reshetnikov/saint-george-on-a-bike/about/research> , <https://zenodo.org/record/6984525> ;
    dcat:distribution [
      a dcat:Distribution ;
      dcat:accessURL <https://zenodo.org/record/6984525> ;
      dcatap:availability <http://data.europa.eu/r5r/stable> ;
      dct:title "Image descriptions"@en ;
      dct:description "A CSV file exported from Zooniverse with some changes. The user information has been anonymized and some non-informative fields were removed. The CSV also includes a field with the filename of the annotated image in the DEArt dataset. Please consult the Zooniverse documentation about the CSV data format."@en ;
      dct:format <http://publications.europa.eu/resource/authority/file-type/CSV> ;
      dct:license <https://creativecommons.org/licenses/by-nc-sa/2.0/> ;
      dcat:mediaType <https://www.iana.org/assignments/media-types/text/csv> ;
	  dct:rights <https://creativecommons.org/licenses/by-nc-sa/2.0/> ;
      adms:status <http://purl.org/adms/status/Completed>
    ] .
  
<https://saintgeorgeonabike.eu/> a foaf:Agent, vcard:Kind ;
  dct:type <http://purl.org/adms/publishertype/NonProfitOrganisation> ;
  foaf:name "Project Saint George on a Bike"@en .
  
<https://creativecommons.org/licenses/by-nc-sa/2.0/>
  a dct:LicenseDocument , dct:RightsStatement;
  dct:type <http://purl.org/adms/licencetype/Attribution> , <http://purl.org/adms/licencetype/NonCommercialUseOnly>, <http://purl.org/adms/licencetype/ViralEffect-ShareAlike>.

<http://purl.org/adms/licencetype/Attribution>
  a skos:Concept ;
  skos:inScheme <http://purl.org/adms/licencetype/1.0> ;
  skos:prefLabel "Attribution"@en .
  
<http://purl.org/adms/licencetype/NonCommercialUseOnly>
  a skos:Concept ;
  skos:inScheme <http://purl.org/adms/licencetype/1.0> ;
  skos:prefLabel "Non-commercial use only"@en .
  
<http://purl.org/adms/licencetype/ViralEffect-ShareAlike>
  a skos:Concept ;
  skos:inScheme <http://purl.org/adms/licencetype/1.0> ;
  skos:prefLabel "Viral effect (a.k.a. Share-alike)"@en .

<https://www.iana.org/assignments/media-types/text/csv>  
  a dct:MediaType .
  
<http://www.iana.org/assignments/media-types/text/html>
  a dct:MediaType .  
  
<http://publications.europa.eu/resource/authority/data-theme> 
  a skos:ConceptScheme ;
  dct:title "Data theme"@en . 
 
<http://publications.europa.eu/resource/authority/data-theme/EDUC>  
  a skos:Concept ;
  skos:inScheme <http://publications.europa.eu/resource/authority/data-theme> ;
  skos:prefLabel "Education"@en . 
  
<http://publications.europa.eu/resource/authority/access-right/PUBLIC>
  a dct:RightsStatement .  
  
<http://purl.org/adms/publishertype/NonProfitOrganisation>
  a skos:Concept ;
  skos:prefLabel "Non-Profit Organisation"@en ; 
  skos:inScheme <http://purl.org/adms/publishertype/1.0> .

<http://publications.europa.eu/resource/authority/file-type/CSV>
  a dct:MediaTypeOrExtent ;
  skos:inScheme <http://publications.europa.eu/resource/authority/file-type> .

<https://zenodo.org/record/6984525>  
  a foaf:Document ;
  schema:url "https://zenodo.org/record/6984525" ;
  dct:title "The dataset landing page at Zenodo."@en ; 
  dct:description "The landing page of the dataset at Zenodo, where the dataset can be accessed."@en ; 
  dct:format <http://publications.europa.eu/resource/authority/file-type/HTML> ;
  dcat:mediaType <http://www.iana.org/assignments/media-types/text/html> ;
  dct:type <http://publications.europa.eu/resource/authority/documentation-type/DOCUMENTATION_MAIN> .

<https://help.zooniverse.org/next-steps/data-exports/>
  a foaf:Document ;
  schema:url "https://help.zooniverse.org/next-steps/data-exports/" ;
  dct:title "Description of the CSV data"@en ; 
  dct:description "Documentation from Zooniverse about the format of its CSV data exports."@en ; 
  dct:format <http://publications.europa.eu/resource/authority/file-type/HTML> ;
  dcat:mediaType <http://www.iana.org/assignments/media-types/text/html> ;
  dct:type <http://publications.europa.eu/resource/authority/documentation-type/DOCUMENTATION_MAIN> .

<https://www.zooniverse.org/projects/artem-dot-reshetnikov/saint-george-on-a-bike/about/research>
  a foaf:Document ;
  schema:url "https://help.zooniverse.org/next-steps/data-exports/" ;
  dct:title "Description of the Zooniverse campaign"@en ; 
  dct:description "Description of the Zooniverse campaign that gave origin to this dataset."@en ; 
  dct:format <http://publications.europa.eu/resource/authority/file-type/HTML> ;
  dcat:mediaType <http://www.iana.org/assignments/media-types/text/html> ;
  dct:type <http://publications.europa.eu/resource/authority/documentation-type/DOCUMENTATION_MAIN> .
