@prefix dcat:   <http://www.w3.org/ns/dcat#> .
@prefix dct:     <http://purl.org/dc/terms/> .
@prefix xsd:    <http://www.w3.org/2001/XMLSchema#> .
@prefix foaf:   <http://xmlns.com/foaf/0.1/> .
@prefix vcard:  <http://www.w3.org/2006/vcard/ns#> .
@prefix adms:   <http://www.w3.org/ns/adms> .
@prefix schema: <http://schema.org/> .
@prefix dcatap: <http://data.europa.eu/r5r/> .
@prefix skos:   <http://www.w3.org/2004/02/skos/core#> .

@prefix :       <http://data.europeana.eu> .

<https://saintgeorgeonabike.eu/dataset/Rijskmuseum>  
    a dcat:Dataset ;
    dct:description "A dataset containing annotations made on images of cultural heritage digital objects from the Rijskmuseum. The annotations resulted from the application of automatic object detection techniques."@en ; 
    dct:title "Object detection annotations on images from the Rijskmuseum"@en ;
    dct:publisher <https://saintgeorgeonabike.eu/> ;
	dcat:contactPoint <http://data.europeana.eu/organization/1482250000001617026> ;
	dct:accessRights <http://publications.europa.eu/resource/authority/access-right/PUBLIC> ;
    dcat:theme <http://publications.europa.eu/resource/authority/data-theme/EDUC> ;
    dct:creator <https://saintgeorgeonabike.eu/> ;
    dct:conformsTo <https://www.w3.org/TR/annotation-model/> ;
    dct:issued "2022-10-01"^^xsd:date ;
	dct:modified "2022-10-01"^^xsd:date ;
    dcat:keyword "culture"@en ;
    foaf:page <https://saintgeorgeonabike.eu/results/dataset/rijskmuseum> ;  
    dcat:distribution [
      a dcat:Distribution ;
      dcat:accessURL <https://saintgeorgeonabike.eu/results/dataset/rijskmuseum> ;
      dcat:downloadURL <https://saintgeorgeonabike.eu/results/dataset/rijskmuseum/downloads/annotations.zip> ;
      dcatap:availability <http://data.europa.eu/r5r/stable> ;
      dct:title "Object detection annotations. (JSON-LD data dumps)"@en ;
      dct:description "A ZIP archive containing the enrichments (as annotations) automatically created by the SGoaB service for a dataset."@en ;
      dct:format <http://publications.europa.eu/resource/authority/file-type/JSON_LD> ;
      dct:license <http://creativecommons.org/publicdomain/zero/1.0/> ;
      dct:conformsTo <https://www.w3.org/TR/annotation-model/> ;
      dcat:mediaType <https://www.iana.org/assignments/media-types/application/ld+json> ;
      dcat:packageFormat <https://www.iana.org/assignments/media-types/application/zip> ;
	  dct:rights <http://creativecommons.org/publicdomain/zero/1.0/> ;  
      adms:status <http://purl.org/adms/status/Completed>
    ] .

<http://data.europeana.eu/organization/1482250000001617026> 
  a foaf:Agent , vcard:Kind ;
  foaf:name "Europeana Foundation"@en, "Stichting Europeana"@nl ;
  dct:type <http://purl.org/adms/publishertype/NonProfitOrganisation> .
  
<https://saintgeorgeonabike.eu/> a foaf:Agent ;
  foaf:name "Project Saint George on a Bike"@en .
  
<http://creativecommons.org/publicdomain/zero/1.0/>
  a dct:LicenseDocument , dct:RightsStatement;
  dct:type <http://purl.org/adms/licencetype/PublicDomain> .

<http://purl.org/adms/licencetype/PublicDomain>
  a skos:Concept ;
  skos:inScheme <http://purl.org/adms/licencetype/1.0> ;
  skos:prefLabel "Public domain"@en .
    
<http://www.europeana.eu/schemas/edm/>  
  a dct:Standard .
  
<https://www.w3.org/TR/annotation-model/>  
  a dct:Standard .
     
<https://www.iana.org/assignments/media-types/text/turtle>
  a dct:MediaType .
  
<https://www.iana.org/assignments/media-types/application/zip>  
  a dct:MediaType .
  
<https://www.iana.org/assignments/media-types/application/ld+json>  
  a dct:MediaType .
  
<http://www.iana.org/assignments/media-types/text/html>
  a dct:MediaType .  
  
<http://publications.europa.eu/resource/authority/file-type/RDF_TURTLE>
  a dct:MediaTypeOrExtent ;
  skos:inScheme <http://publications.europa.eu/resource/authority/file-type> .

<http://publications.europa.eu/resource/authority/file-type/HTML>   
  a dct:MediaTypeOrExtent ;
  skos:inScheme <http://publications.europa.eu/resource/authority/file-type> .
    
<http://publications.europa.eu/resource/authority/file-type/JSON_LD>
  a dct:MediaTypeOrExtent ;
  skos:inScheme <http://publications.europa.eu/resource/authority/file-type> .

<http://publications.europa.eu/resource/authority/data-theme> 
  a skos:ConceptScheme ;
  dct:title "Data theme"@en . 
 
<http://publications.europa.eu/resource/authority/data-theme/EDUC>  
  a skos:Concept ;
  skos:inScheme <http://publications.europa.eu/resource/authority/data-theme> ;
  skos:prefLabel "Education"@en . 
  
<http://publications.europa.eu/resource/authority/access-right/PUBLIC>
  a dct:RightsStatement .  
  
<http://purl.org/adms/publishertype/NonProfitOrganisation>
  a skos:Concept ;
  skos:prefLabel "Non-Profit Organisation"@en ; 
  skos:inScheme <http://purl.org/adms/publishertype/1.0> .
  
<https://saintgeorgeonabike.eu/results/dataset/rijskmuseum>  
  a foaf:Document ;
  schema:url "https://saintgeorgeonabike.eu/results/dataset/rijskmuseum" ;
  dct:title "Instructions for using and downloading the dataset"@en ; 
  dct:description "Instructions for using and downloading the object detection annotations on images from the Rijskmuseum."@en ; 
  dct:format <http://publications.europa.eu/resource/authority/file-type/HTML> ;
  dcat:mediaType <http://www.iana.org/assignments/media-types/text/html> ;
  dct:type <http://publications.europa.eu/resource/authority/documentation-type/DOCUMENTATION_MAIN> .

<https://pro.europeana.eu/page/edm-documentation>
  a foaf:Document ;
  schema:url "https://pro.europeana.eu/page/edm-documentation" ;
  dct:title "Documentation about the Europeana Data Model"@en ; 
  dct:description "This webpage list all the documentation resources required for creating and using data in the Europeana Data Model format."@en ; 
  dct:format <http://publications.europa.eu/resource/authority/file-type/HTML> ;
  dcat:mediaType <http://www.iana.org/assignments/media-types/text/html> ;
  dct:type <http://publications.europa.eu/resource/authority/documentation-type/DOCUMENTATION_MAIN> .




